SP1Operations/CPUState.lean
@@ -1,37 +1,32 @@
 import SP1Foundations
 
--- CPUState is not parameterized by a type `T` because there shouldn't be a case
--- where we want dynamically enforce the size of `shard`, `clk`, and `pc`. In
--- other words, it shouldn't happen that sometimes we want to enfroce `pc` as U8
--- and sometimes we want to enforce `pc` as U16. They should really just be
--- `BabyBear`.
 structure CPUState where
-  shard : BabyBear
-  clk_high_limb : BabyBear
-  clk_low_limb : BabyBear
-  pc : BabyBear
+  clk_high: BabyBear
+  clk_16_24: BabyBear
+  clk_0_16: BabyBear
+  pc: BabyBear
 
 namespace CPUState
 
-def clk (cols : CPUState) : BabyBear := 2^14 * cols.clk_high_limb + cols.clk_low_limb
+def clk (cols : CPUState) : BabyBear := sorry --2^14 * cols.clk_high_limb + cols.clk_low_limb
 
 def constraints
   (cols : CPUState)
   (next_pc : BabyBear)
   (clk_increment : BabyBear)
   (is_real : BabyBear)
-  : List SP1Constraint :=
-  let E0 : BabyBear := 16384 * cols.clk_high_limb
-  let E2 : BabyBear := E0 + cols.clk_low_limb
-  let E4 : BabyBear := is_real - 1
-  let E6 : BabyBear := is_real * E4
-  let E8 : BabyBear := E2 + clk_increment
-  [
-    .assertZero E6,
-    .receive (.state cols.shard E2 cols.pc) is_real,
-    .send (.state cols.shard E8 next_pc) is_real,
-    .send (.byte ByteOpcode.Range cols.clk_high_limb 14 0) is_real,
-    .send (.byte ByteOpcode.Range cols.clk_low_limb 14 0) is_real
-  ]
+  : List SP1Constraint := []
+  -- let E0 : BabyBear := 16384 * cols.clk_high_limb
+  -- let E2 : BabyBear := E0 + cols.clk_low_limb
+  -- let E4 : BabyBear := is_real - 1
+  -- let E6 : BabyBear := is_real * E4
+  -- let E8 : BabyBear := E2 + clk_increment
+  -- [
+  --   .assertZero E6,
+  --   .receive (.state cols.shard E2 cols.pc) is_real,
+  --   .send (.state cols.shard E8 next_pc) is_real,
+  --   .send (.byte ByteOpcode.Range cols.clk_high_limb 14 0) is_real,
+  --   .send (.byte ByteOpcode.Range cols.clk_low_limb 14 0) is_real
+  -- ]
 
 end CPUState
