SP1Operations/RTypeReader.lean
@@ -33,21 +33,21 @@ def constraints
   let E16 : BabyBear := clk + 3
   let E18 : BabyBear := is_real - 1
   let E20 : BabyBear := is_real * E18
-  let E22 : BabyBear := E16 - cols.op_a_memory.access_timestamp.prev_clk
+  let E22 : BabyBear := E16 - cols.op_a_memory.access_timestamp.prev_low
   let E24 : BabyBear := E22 - 1
   let E26 : BabyBear := E24 - cols.op_a_memory.access_timestamp.diff_low_limb
   let E28 : BabyBear := E26 * 2013143041
   let E30 : BabyBear := clk + 2
   let E32 : BabyBear := is_real - 1
   let E34 : BabyBear := is_real * E32
-  let E36 : BabyBear := E30 - cols.op_b_memory.access_timestamp.prev_clk
+  let E36 : BabyBear := E30 - cols.op_b_memory.access_timestamp.prev_low
   let E38 : BabyBear := E36 - 1
   let E40 : BabyBear := E38 - cols.op_b_memory.access_timestamp.diff_low_limb
   let E42 : BabyBear := E40 * 2013143041
   let E44 : BabyBear := clk + 1
   let E46 : BabyBear := is_real - 1
   let E48 : BabyBear := is_real * E46
-  let E50 : BabyBear := E44 - cols.op_c_memory.access_timestamp.prev_clk
+  let E50 : BabyBear := E44 - cols.op_c_memory.access_timestamp.prev_low
   let E52 : BabyBear := E50 - 1
   let E54 : BabyBear := E52 - cols.op_c_memory.access_timestamp.diff_low_limb
   let E56 : BabyBear := E54 * 2013143041
@@ -59,17 +59,17 @@ def constraints
     .assertZero E20,
     .send (.byte ByteOpcode.Range cols.op_a_memory.access_timestamp.diff_low_limb 14 0) is_real,
     .send (.byte ByteOpcode.Range E28 14 0) is_real,
-    .send (.memory shard cols.op_a_memory.access_timestamp.prev_clk cols.op_a cols.op_a_memory.prev_value[0] cols.op_a_memory.prev_value[1]) is_real,
+    .send (.memory shard cols.op_a_memory.access_timestamp.prev_low cols.op_a cols.op_a_memory.prev_value[0] cols.op_a_memory.prev_value[1]) is_real,
     .receive (.memory shard E16 cols.op_a op_a_write_value[0] op_a_write_value[1]) is_real,
     .assertZero E34,
     .send (.byte ByteOpcode.Range cols.op_b_memory.access_timestamp.diff_low_limb 14 0) is_real,
     .send (.byte ByteOpcode.Range E42 14 0) is_real,
-    .send (.memory shard cols.op_b_memory.access_timestamp.prev_clk cols.op_b cols.op_b_memory.prev_value[0] cols.op_b_memory.prev_value[1]) is_real,
+    .send (.memory shard cols.op_b_memory.access_timestamp.prev_low cols.op_b cols.op_b_memory.prev_value[0] cols.op_b_memory.prev_value[1]) is_real,
     .receive (.memory shard E30 cols.op_b cols.op_b_memory.prev_value[0] cols.op_b_memory.prev_value[1]) is_real,
     .assertZero E48,
     .send (.byte ByteOpcode.Range cols.op_c_memory.access_timestamp.diff_low_limb 14 0) is_real,
     .send (.byte ByteOpcode.Range E56 14 0) is_real,
-    .send (.memory shard cols.op_c_memory.access_timestamp.prev_clk cols.op_c cols.op_c_memory.prev_value[0] cols.op_c_memory.prev_value[1]) is_real,
+    .send (.memory shard cols.op_c_memory.access_timestamp.prev_low cols.op_c cols.op_c_memory.prev_value[0] cols.op_c_memory.prev_value[1]) is_real,
     .receive (.memory shard E44 cols.op_c cols.op_c_memory.prev_value[0] cols.op_c_memory.prev_value[1]) is_real
   ]
 
